lib/Marshalling/MarshalledAccessors.i.dfy
@@ -1,76 +1,492 @@
-include "GenericMarshalling.i.dfy"
+include "../Lang/NativeTypes.s.dfy"
+include "../Lang/System/PackedInts.s.dfy"
+//include "../Lang/LinearSequence.s.dfy"
+include "../Base/Option.s.dfy"
+include "../Base/mathematics.i.dfy"
 
-module MarshalledAccessors {
-  import opened GenericMarshalling`Internal
+abstract module Marshalling {
   import opened NativeTypes
-  import opened NativePackedInts
-  import opened Sequences
-
-  datatype MarshalledUint32Array = MarshalledUint32Array(data: seq<byte>, start: uint64)
-  {
-    predicate WF() {
-      && |data| < Uint64UpperBound()
-      && start as int <= |data|
-      && parse_Uint32Array(data[start..]).0.Some?
-    }
-
-    function I() : seq<uint32>
-      requires WF()
-    {
-      parse_Uint32Array(data[start..]).0.value.va
-    }
+  import opened Options
   
-    method Length() returns (length: uint64)
-    requires WF()
-    ensures length as int == |I()|
-    {
-      length := Unpack_LittleEndian_Uint64(data[start..], 0);
-    }
+  type UnmarshalledType
 
-    method Size() returns (size: uint64)
-      requires WF()
-      ensures size as int == SizeOfV(VUint32Array(I()))
-    {
-      var length := Length();
-      size := 8 + 4 * length;
-    }
-  
-    method Element(i: uint64) returns (element: uint32)
-      requires WF()
-      requires i as int < |I()|
-      ensures element == I()[i]
-    {
-      var idx := 8 + i * 4;
-      element := Unpack_LittleEndian_Uint32(data, start + idx);
+  // "mseq" == "machine seq"
+  type mseq<T> = s : seq<T> | |s| < Uint64UpperBound()
 
-      ghost var len := |parse_Uint32Array(data[start..]).0.value.va|;
+  predicate parsable(data: mseq<byte>)
+
+  function parse(data: mseq<byte>) : UnmarshalledType
+    requires parsable(data)
+
+  method TryParse(data: mseq<byte>) returns (ovalue: Option<UnmarshalledType>)
+    ensures parsable(data) <==> ovalue.Some?
+    ensures parsable(data) ==> ovalue.value == parse(data)
     
-      calc {
-        element;
-        unpack_LittleEndian_Uint32(data[start + idx..start + idx + 4]);
-        { lemma_seq_suffix_slice(data, start as int, idx as int, idx as int + 4); }
-        unpack_LittleEndian_Uint32(data[start..][idx..idx + 4]);
-        unpack_LittleEndian_Uint32(data[start..][8 + i * 4..8 + i * 4 + 4]);
-        { lemma_seq_suffix_slice(data[start..], 8, i as int * 4, i as int * 4 + 4); }
-        unpack_LittleEndian_Uint32(data[start..][8..][i * 4..i * 4 + 4]);
-        { lemma_seq_extensionality_slice(data[start..][8..], data[start..][8..][..len*4], i as int * 4, i as int * 4 + 4); }
-        unpack_LittleEndian_Uint32(data[start..][8..][..len*4][i * 4..i * 4 + 4]);
-        unpack_LittleEndian_Uint32_Seq(data[start..][8..][0..4*len], len as int)[i];
-        { lemma_seq_suffix_slice(data[start..], 8, 0, 4*len); }
-        unpack_LittleEndian_Uint32_Seq(data[start..][8..8+4*len], len as int)[i];
-        parse_Uint32Array(data[start..]).0.value.va[i];
-      }
+  // FIXME: robj: Would like to provide this as default implementations,
+  // but overriding in in refining modules gives an error about
+  // assigning to p.
+  method Parsable(data: mseq<byte>) returns (p: bool)
+    ensures p == parsable(data)
+  // {
+  //   var ovalue := TryParse(data);
+  //   p := ovalue.Some?;
+  // }
+  
+  // FIXME: robj: Would like to provide this as default
+  // implementations, but overriding in in refining modules gives an
+  // error about assigning to p.
+  method Parse(data: mseq<byte>) returns (value: UnmarshalledType)
+    requires parsable(data)
+    ensures value == parse(data)
+  // {
+  //   var ovalue := TryParse(data);
+  //   value := ovalue.value;
+  // }
+
+  predicate marshallable(value: UnmarshalledType)
+    
+  function size(value: UnmarshalledType) : nat
+    requires marshallable(value)
+
+  method Size(value: UnmarshalledType) returns (sz: uint64)
+    requires marshallable(value)
+    requires size(value) < Uint64UpperBound()
+    ensures sz as nat == size(value)
+
+  // FIXME: robj: data should be linear inout doesn't work with module
+  // refinement.
+  method Marshall(value: UnmarshalledType, linear data: mseq<byte>, start: uint64)
+    returns (linear newdata: mseq<byte>, end: uint64)
+    requires marshallable(value)
+    requires start as nat + size(value) <= |data|
+    ensures end as nat == start as nat + size(value)
+    ensures |newdata| == |data|
+    ensures forall i | 0 <= i < start :: newdata[i] == data[i]
+    ensures forall i | end <= i < |newdata| as uint64 :: newdata[i] == data[i]
+    ensures parsable(newdata[start..end])
+    ensures parse(newdata[start..end]) == value
+}
+
+abstract module IntegerMarshalling refines Marshalling {
+  import Int : NativePackedInt
+    
+  type UnmarshalledType = Int.Integer
+
+  predicate parsable(data: mseq<byte>)
+  {
+    Int.Size() as nat <= |data|
+  }
+
+  function parse(data: mseq<byte>) : UnmarshalledType
+  {
+    Int.unpack(data[..Int.Size()])
+  }
+      
+  method TryParse(data: mseq<byte>) returns (ovalue: Option<UnmarshalledType>)
+  {
+    if Int.Size() <= |data| as uint64 {
+      var value := Int.Unpack(data, 0);
+      ovalue := Some(value);
+    } else {
+      ovalue := None;
     }
   }
 
-  method ByteArraySlice(data: seq<byte>, start: uint64, from: uint64, to: uint64)
-    returns (s: seq<byte>)
-    requires |data| < Uint64UpperBound()
-    requires start as int <= |data|
-    requires parse_ByteArray(data[start..]).0.Some?
-    requires from as int <= to as int <= |parse_ByteArray(data[start..]).0.value.b|
-    ensures s == parse_ByteArray(data[start..]).0.value.b[from..to]
+  method Parsable(data: mseq<byte>) returns (p: bool)
   {
-    s := data[start + 8 + from..start + 8+ to];
-  }    
+    p := Int.Size() <= |data| as uint64;
+  }
+  
+  method Parse(data: mseq<byte>) returns (value: UnmarshalledType)
+  {
+    value := Int.Unpack(data, 0);
+  }
+
+  predicate marshallable(value: UnmarshalledType) {
+    true
+  }
+      
+  function size(value: UnmarshalledType) : nat
+  {
+    Int.Size() as nat
+  }
+  
+  method Size(value: UnmarshalledType) returns (sz: uint64)
+  {
+    sz := Int.Size();
+  }
+  
+  method Marshall(value: UnmarshalledType, linear data: mseq<byte>, start: uint64)
+    returns (linear newdata: mseq<byte>, end: uint64)
+  {
+      newdata := data;
+      Int.Pack_into_ByteSeq(value, inout newdata, start);
+      end := start + Int.Size();
+      assert newdata[start..end][..Int.Size()] == newdata[start..start + Int.Size()];
+  }
 }
+
+module Uint32Marshalling refines IntegerMarshalling {
+  import Int = NativePackedUint32
+}
+
+module Uint64Marshalling refines IntegerMarshalling {
+  import Int = NativePackedUint64
+}
+
+abstract module SeqMarshalling refines Marshalling {
+  import ElementMarshalling : Marshalling
+
+  type Element = ElementMarshalling.UnmarshalledType
+  type UnmarshalledType = mseq<Element>
+
+  predicate lengthable(data: mseq<byte>)
+    ensures parsable(data) ==> lengthable(data)
+
+  method TryLength(data: mseq<byte>) returns (olen: Option<uint64>)
+    ensures lengthable(data) <==> olen.Some?
+    ensures parsable(data) ==> olen.value as nat == |parse(data)|
+
+  method Lengthable(data: mseq<byte>) returns (l: bool)
+    ensures l == lengthable(data)
+    
+  method Length(data: mseq<byte>) returns (len: uint64)
+    requires lengthable(data)
+    ensures parsable(data) ==> len as nat == |parse(data)|
+
+
+  predicate gettable(data: mseq<byte>, idx: nat)
+    ensures parsable(data) && idx < |parse(data)| ==> gettable(data, idx)
+
+  method TryGet(data: mseq<byte>, idx: uint64) returns (oedata: Option<mseq<byte>>)
+    ensures oedata.Some? <==> gettable(data, idx as nat)
+    ensures parsable(data) && |parse(data)| <= idx as nat ==> oedata.None?
+    ensures parsable(data) && idx as nat < |parse(data)| ==> ElementMarshalling.parsable(oedata.value)
+    ensures parsable(data) && idx as nat < |parse(data)| ==> ElementMarshalling.parse(oedata.value) == parse(data)[idx]
+
+  method Gettable(data: mseq<byte>, idx: uint64) returns (g: bool)
+    ensures g == gettable(data, idx as nat)
+
+
+  method Get(data: mseq<byte>, idx: uint64) returns (edata: mseq<byte>)
+    requires gettable(data, idx as nat)
+    ensures parsable(data) && idx as nat < |parse(data)| ==> ElementMarshalling.parsable(edata)
+    ensures parsable(data) && idx as nat < |parse(data)| ==> ElementMarshalling.parse(edata) == parse(data)[idx]
+}
+
+abstract module IntegerSeqMarshalling refines SeqMarshalling {
+  import ElementMarshalling = IntegerMarshalling
+  import Int = ElementMarshalling.Int
+    
+  predicate lengthable(data: mseq<byte>)
+  {
+    true
+  }
+
+  function length(data: mseq<byte>) : nat
+  {
+    |data| / Int.Size() as nat
+  }
+  
+  method TryLength(data: mseq<byte>) returns (olen: Option<uint64>)
+  {
+    var dlen := |data| as uint64;
+    olen := Some(dlen / Int.Size());
+  }
+
+  method Lengthable(data: mseq<byte>) returns (l: bool)
+  {
+    l := true;
+  }
+  
+  method Length(data: mseq<byte>) returns (len: uint64)
+  {
+    len := |data| as uint64 / Int.Size();
+  }
+
+  predicate parsable(data: mseq<byte>)
+  {
+    true
+  }
+
+  function parse(data: mseq<byte>) : UnmarshalledType
+  {
+    var length := length(data);
+    Int.unpack_Seq(data[..length * Int.Size() as nat], length)
+  }
+
+  method TryParse(data: mseq<byte>) returns (ovalue: Option<UnmarshalledType>)
+  {
+    var length := Length(data);
+    var value := Int.Unpack_Seq(data, 0, length);
+    assert |value| < Uint64UpperBound();
+    ovalue := Some(value);
+  }
+
+  method Parsable(data: mseq<byte>) returns (p: bool)
+  {
+    p := true;
+  }
+
+  method Parse(data: mseq<byte>) returns (value: UnmarshalledType)
+  {
+    var length := Length(data);
+    value := Int.Unpack_Seq(data, 0, length);
+  }
+  
+  predicate gettable(data: mseq<byte>, idx: nat)
+  {
+    idx < length(data)
+  }
+
+  lemma GetCorrect(data: mseq<byte>, idx: uint64)
+    requires idx as nat < length(data)
+    ensures idx as nat * Int.Size() as nat + Int.Size() as nat <= |data|
+    ensures ElementMarshalling.parse(data[idx * Int.Size()..idx * Int.Size() + Int.Size()]) == parse(data)[idx]
+  {
+    //assert idx as nat + 1 <= length(data);
+    assert (idx as nat + 1) * Int.Size() as nat <= length(data) * Int.Size() as nat;
+    assert length(data) * Int.Size() as nat <= (|data| / Int.Size() as nat) * Int.Size() as nat;
+    calc {
+      ElementMarshalling.parse(data[idx * Int.Size()..idx * Int.Size() + Int.Size()]);
+      Int.unpack(data[idx * Int.Size()..(idx + 1) * Int.Size()][..Int.Size()]);
+      Int.unpack(data[idx * Int.Size()..(idx + 1) * Int.Size()][0..Int.Size()]);
+      { assert data[idx * Int.Size()..(idx + 1) * Int.Size()][..Int.Size()] == data[idx * Int.Size()..idx * Int.Size() + Int.Size()]; }
+      Int.unpack(data[idx * Int.Size()..idx * Int.Size() + Int.Size()]);
+      Int.unpack(data[idx as nat * Int.Size() as nat.. (idx as nat + 1) * Int.Size() as nat]);
+      { assert data[..length(data) * Int.Size() as nat][idx as nat * Int.Size() as nat.. (idx as nat + 1) * Int.Size() as nat] == data[idx as nat * Int.Size() as nat.. (idx as nat + 1) * Int.Size() as nat]; }
+      Int.unpack(data[..length(data) * Int.Size() as nat][idx as nat * Int.Size() as nat.. (idx as nat + 1) * Int.Size() as nat]);
+      Int.unpack_Seq(data[..length(data) * Int.Size() as nat], length(data))[idx];
+      parse(data)[idx];
+    }
+  }
+  
+  method TryGet(data: mseq<byte>, idx: uint64) returns (oedata: Option<mseq<byte>>)
+  {
+    var len := Length(data);
+    if idx < len {
+      GetCorrect(data, idx);
+      oedata := Some(data[idx * Int.Size()..idx * Int.Size() + Int.Size()]);
+    } else {
+      oedata := None;
+    }
+  }
+  
+  method Gettable(data: mseq<byte>, idx: uint64) returns (g: bool)
+  {
+    var len := Length(data);
+    g := idx < len;
+  }
+
+  method Get(data: mseq<byte>, idx: uint64) returns (edata: mseq<byte>)
+  {
+    var len := Length(data);
+    if idx < len {
+      GetCorrect(data, idx);
+      edata := data[idx * Int.Size()..idx * Int.Size() + Int.Size()];
+    } else {
+      edata := [];
+    }
+  }
+
+  method FastGet(data: mseq<byte>, idx: uint64) returns (element: Element)
+    requires idx as nat < length(data)
+    ensures element == parse(data)[idx]
+  {
+    GetCorrect(data, idx);
+    element := Int.Unpack(data, idx * Int.Size());
+    assert data[idx * Int.Size()..idx * Int.Size() + Int.Size()] == data[idx * Int.Size()..idx * Int.Size() + Int.Size()][..Int.Size()];
+  }
+}
+
+// FIXME: Can't instantiate these with current limitations of module
+// system.
+
+// module Uint32SeqMarshalling refines IntegerSeqMarshalling {
+// }
+
+// module Uint64SeqMarshalling refines IntegerSeqMarshalling {
+//   import Int = NativePackedUint64
+// }
+
+
+abstract module UniformSizedElementSeqMarshalling refines SeqMarshalling {
+  import opened Mathematics
+  function method UniformSize() : uint64
+    ensures 0 < UniformSize()
+
+  predicate lengthable(data: mseq<byte>)
+  {
+    true
+  }
+
+  function length(data: mseq<byte>) : nat
+  {
+    |data| / UniformSize() as nat
+  }
+  
+  method TryLength(data: mseq<byte>) returns (olen: Option<uint64>)
+  {
+    assert |data| / UniformSize() as nat <= |data|;
+    olen := Some(|data| as uint64 / UniformSize());
+  }
+  
+  method Lengthable(data: mseq<byte>) returns (l: bool)
+  {
+    l := true;
+  }
+  
+  method Length(data: mseq<byte>) returns (len: uint64)
+    ensures len as nat == length(data)
+  {
+    assert |data| / UniformSize() as nat <= |data|;
+    len := |data| as uint64 / UniformSize();
+  }
+  
+  function method ElementData(data: mseq<byte>, idx: uint64) : mseq<byte>
+    requires idx as nat < length(data)
+  {
+    DivMulOrder(length(data), UniformSize() as nat);
+    assert (idx as nat + 1) * UniformSize() as nat <= |data|;
+    assert (idx as nat + 1) * UniformSize() as nat == idx as nat * UniformSize() as nat + UniformSize() as nat;
+    data[idx * UniformSize()..idx * UniformSize() + UniformSize()]
+  }
+
+  predicate parsable(data: mseq<byte>) {
+    forall idx | 0 <= idx < length(data) :: ElementMarshalling.parsable(ElementData(data, idx as uint64))
+  }
+
+  function parse_prefix(data: mseq<byte>, len: nat) : (result: UnmarshalledType)
+    requires parsable(data)
+    requires len <= length(data)
+    ensures |result| == len
+    ensures forall i | 0 <= i < len :: result[i] == ElementMarshalling.parse(ElementData(data, i as uint64))
+  {
+    if len == 0 then
+      []
+    else
+      var prefix := parse_prefix(data, len - 1);
+      var last := ElementMarshalling.parse(ElementData(data, len as uint64 - 1));
+      prefix + [last]
+  }
+
+  function parse(data: mseq<byte>) : (result: UnmarshalledType)
+  {
+    var len := length(data);
+    parse_prefix(data, len)
+  }
+
+  predicate gettable(data: mseq<byte>, idx: nat)
+  {
+    idx < length(data)
+  }
+  
+  method TryGet(data: mseq<byte>, idx: uint64) returns (oedata: Option<mseq<byte>>)
+  {
+    var len := Length(data);
+    if idx < len {
+      oedata := Some(ElementData(data, idx));
+    } else {
+      oedata := None;
+    }
+  }
+
+  method Gettable(data: mseq<byte>, idx: uint64) returns (g: bool)
+  {
+    var len := Length(data);
+    g := idx < len;
+  }
+
+  method Get(data: mseq<byte>, idx: uint64) returns (edata: mseq<byte>)
+  {
+    edata := ElementData(data, idx);
+  }
+
+
+  predicate marshallable(value: UnmarshalledType)
+  {
+    && (forall i | 0 <= i < |value| :: ElementMarshalling.marshallable(value[i]))
+    && (forall i | 0 <= i < |value| :: ElementMarshalling.size(value[i]) == UniformSize() as nat)
+  }
+
+  lemma marshallable_prefix(value: UnmarshalledType, len: nat)
+    requires marshallable(value)
+    requires 0 <= len <= |value|
+    ensures marshallable(value[..len])
+  {
+  }
+
+  function size(value: UnmarshalledType) : nat
+  {
+    |value| * UniformSize() as nat
+  }
+
+  method Size(value: UnmarshalledType) returns (sz: uint64)
+  {
+    sz := |value| as uint64 * UniformSize();
+  }
+
+  lemma parsing_extend(data: mseq<byte>, edata: mseq<byte>)
+    requires parsable(data)
+    requires |data| == length(data) * UniformSize() as nat
+    requires ElementMarshalling.parsable(edata)
+    requires |edata| == UniformSize() as nat
+    ensures parsable(data + edata)
+    ensures parse(data + edata) == parse(data) + [ ElementMarshalling.parse(edata) ]
+  {
+    var extension := data + edata;
+    calc {
+      length(extension);
+      |extension| / UniformSize() as nat;
+      (|data| + UniformSize() as nat) / UniformSize() as nat;
+      |data| / UniformSize() as nat + UniformSize() as nat / UniformSize() as nat;
+      |data| / UniformSize() as nat + 1;
+      length(data) + 1;
+    }
+    forall idx | 0 <= idx < length(extension)
+      ensures ElementMarshalling.parsable(ElementData(extension, idx as uint64))
+      ensures idx < length(data) ==> parse(extension)[idx] == parse(data)[idx]
+      ensures idx == length(data) ==> parse(extension)[idx] == ElementMarshalling.parse(edata)
+    {
+      if idx < length(data) {
+        assert (idx + 1) * UniformSize() as nat <= length(data) * UniformSize() as nat;
+        assert ElementData(extension, idx as uint64) == ElementData(data, idx as uint64);
+      } else {
+        assert ElementData(extension, idx as uint64) == edata;
+      }
+    }
+  }
+  
+  method Marshall(value: UnmarshalledType, linear data: mseq<byte>, start: uint64)
+    returns (linear newdata: mseq<byte>, end: uint64)
+  {
+    newdata := data;
+    var i: uint64 := 0;
+    end := start;
+    while i < |value| as uint64
+      invariant i <= |value| as uint64
+      invariant |newdata| == |data|
+      invariant end as nat == start as nat + size(value[..i])
+      invariant forall j | 0 <= j < start :: newdata[j] == data[j]
+      invariant forall j | end as nat <= j < |data| :: newdata[j] == data[j]
+      invariant parsable(newdata[start..end])
+      invariant parse(newdata[start..end]) == value[..i]
+    {
+      ghost var oldend := end;
+      ghost var olddata := newdata[start..end];
+      assert i as nat + 1 <= |value|;
+      assert start as nat + (i as nat + 1) * UniformSize() as nat <= start as nat + |value| * UniformSize() as nat;
+
+      newdata, end := ElementMarshalling.Marshall(value[i], newdata, end);
+      i := i + 1;
+
+      assert newdata[start..oldend] == olddata;
+      parsing_extend(newdata[start..oldend], newdata[oldend..end]);
+      assert newdata[start..end] == newdata[start..oldend] + newdata[oldend..end];
+      assert value[..i] == value[..i-1] + [ value[i-1] ];
+    }
+    assert value == value[..|value|];
+  }
+}
+
+
