lib/Marshalling/StaticallySizedMarshalling.i.dfy
@@ -1,160 +1,205 @@
 include "../Lang/NativeTypes.s.dfy"
+include "../Lang/System/PackedInts.s.dfy"
+include "../Base/Option.s.dfy"
 
 module StaticallySizedMarshalling {
-import opened NativeTypes
+  import opened NativeTypes
+  import opened NativePackedInts
+  import opened Options
   
-datatype StaticallySizedGrammar =
-    SSGUint32
-  | SSGUint64
-  | SSGArray(len: nat, elt: StaticallySizedGrammar)
-  | SSGTuple(t: seq<StaticallySizedGrammar>, names: seq<string>)
-  | SSGByteArray(len: nat)
-  | SSGUint32Array(len: nat)
-  | SSGUint64Array(len: nat)
-  | SSGTaggedUnion(cases: seq<StaticallySizedGrammar>, names: seq<string>)
-  | SSGPadded(size: nat, delt: G)   // size: max size in bytes
-    // TODO(robj): what does 'delt' mean?
+  datatype StaticallySizedGrammar =
+    | SSGUint32
+    | SSGUint64
+    | SSGByteArray(len: nat)
+    | SSGUint32Array(len: nat)
+    | SSGUint64Array(len: nat)
+    | SSGTuple(t: seq<StaticallySizedGrammar>)
+    | SSGTaggedUnion(cases: seq<StaticallySizedGrammar>)
+    | SSGPadded(size: nat, delt: DynamicallySizedGrammar)   // size: max size in bytes
+    
+  datatype DynamicallySizedGrammar =
+    | GByteArray
+    | GUint32Array
+    | GUint64Array
+    | GArray(elt:DynamicallySizedGrammar)
+    | GSSArray(selt: StaticallySizedGrammar)
+    | GTuple(t:seq<DynamicallySizedGrammar>)
+    | GTaggedUnion(cases:seq<DynamicallySizedGrammar>)
+
+  datatype StaticallySizedValue = 
+    | SSVUint32(v:uint32)
+    | SSVUint64(u:uint64)
+    | SSVArray(a:seq<StaticallySizedValue>)
+    | SSVTuple(t:seq<StaticallySizedValue>)
+    | SSVByteArray(b:seq<byte>)
+    | SSVUint32Array(va:seq<uint32>)
+    | SSVUint64Array(ua:seq<uint64>)
+    | SSVCase(c:uint64, casev:StaticallySizedValue)
+    | SSVPadded(size: uint64, padv:DynamicallySizedValue)
+
+  datatype DynamicallySizedValue =
+    | StaticallySizedValue(v: StaticallySizedValue)
+    | VArray(a:seq<DynamicallySizedValue>)
+    | VSSArray(sa:seq<StaticallySizedValue>)
+    | VTuple(t:seq<DynamicallySizedValue>)
+    | VByteArray(b:seq<byte>)
+    | VUint32Array(va:seq<uint32>)
+    | VUint64Array(ua:seq<uint64>)
+    | VCase(c:uint64, val:DynamicallySizedValue)
+
+  function SizeOfStaticallySizedGrammarSeq(grammars: seq<StaticallySizedGrammar>) : nat
+  {
+    if |grammars| == 0 then 0
+    else SizeOfStaticallySizedGrammarSeq(grammars[..|grammars|-1]) + SizeOfStaticallySizedGrammar(grammars[|grammars|-1])
+  }
+
+  function MaxStaticallySizedGrammar(grammars: seq<StaticallySizedGrammar>) : nat
+  {
+    if |grammars| == 0 then 0
+    else
+      var prefixMax := SizeOfStaticallySizedGrammarSeq(grammars[..|grammars|-1]);
+      var last := SizeOfStaticallySizedGrammar(grammars[|grammars|-1]);
+      if prefixMax < last then last
+      else prefixMax
+  }
+
+  function SizeOfStaticallySizedGrammar(grammar: StaticallySizedGrammar) : nat
+  {
+    match grammar
+      case SSGUint32 => 4
+      case SSGUint64 => 8
+      case SSGByteArray(len)   => len
+      case SSGUint32Array(len) => 4 * len
+      case SSGUint64Array(len) => 8 * len
+      case SSGTuple(t) =>  SizeOfStaticallySizedGrammarSeq(t)
+      case SSGTaggedUnion(cases) => MaxStaticallySizedGrammar(cases)
+      case SSGPadded(size, delt) => size
+  }
+
+  function SizeOfVSeq(vals: seq<DynamicallySizedValue>, grammar: DynamicallySizedGrammar) : nat
+    requires forall i | 0 <= i < |vals| :: ValInGrammar(vals[i], grammar)
+    decreases grammar, vals, 1
+  {
+    if |vals| == 0 then 0
+    else SizeOfVSeq(vals[..|vals|-1], grammar) + SizeOfV(vals[|vals|-1], grammar)
+  }
+
+  function SizeOfVGSeq(vals: seq<DynamicallySizedValue>, grammars: seq<DynamicallySizedGrammar>) : nat
+    requires |vals| == |grammars|
+    requires forall i | 0 <= i < |vals| :: ValInGrammar(vals[i], grammars[i])
+    decreases grammars, vals, 1
+  {
+    if |vals| == 0 then 0
+    else SizeOfVGSeq(vals[..|vals|-1], grammars[..|grammars|-1]) + SizeOfV(vals[|vals|-1], grammars[|grammars|-1])
+  }
+
+  function SizeOfV(val:DynamicallySizedValue, grammar: DynamicallySizedGrammar) : nat
+    requires ValInGrammar(val, grammar)
+    decreases grammar, val, 1
+  {
+    match grammar
+      case GByteArray          => |val.b|
+      case GUint32Array        => 4 * |val.va|
+      case GUint64Array        => 8 * |val.ua|
+      case GArray(elt)         => 8 + 8 * |val.a| + SizeOfVSeq(val.a, elt)
+      case GSSArray(selt)      => |val.sa| * SizeOfStaticallySizedGrammar(selt)
+      case GTuple(t)           => 8 * |t| + SizeOfVGSeq(val.t, t)
+      case GTaggedUnion(cases) => 8 + SizeOfV(val.val, cases[val.c])
+  }
   
-datatype G = StaticallySizedElement(g: StaticallySizedGrammar)
-           | GArray(elt:G)
-           | GSSArray(selt: StaticallySizedGrammar)
-           | GTuple(t:seq<G>)
-           | GByteArray
-           | GUint32Array
-           | GUint64Array
-           | GTaggedUnion(cases:seq<G>)
+  predicate StaticallySizedValInStaticallySizedGrammar(val:StaticallySizedValue, grammar:StaticallySizedGrammar)
+    decreases grammar, val, 1
+  {
+    match grammar
+      case SSGUint32 => val.SSVUint32?
+      case SSGUint64 => val.SSVUint64?
+      case SSGByteArray(len)   => val.SSVByteArray? && |val.b| == len
+      case SSGUint32Array(len) => val.SSVUint32Array? && |val.va| == len
+      case SSGUint64Array(len) => val.SSVUint64Array? && |val.ua| == len
 
-datatype StaticallySizedValue = 
-           | SSVUint32(v:uint32)
-           | SSVUint64(u:uint64)
-           // what does it even mean for a value to be SS vs DS?
-           | SSVArray(a:seq<StaticallySizedValue>)
-           | SSVTuple(t:seq<StaticallySizedValue>)
-           | SSVByteArray(b:seq<byte>)
-           | SSVUint32Array(va:seq<uint32>)
-           | SSVUint64Array(ua:seq<uint64>)
-           | SSVCase(c:uint64, casev:StaticallySizedValue)
-           | SSVPadded(size: uint64, padv:V)
+      case SSGTuple(t) =>
+        && val.SSVTuple?
+        && |val.t| == |t|
+        && forall i :: 0 <= i < |t| ==> StaticallySizedValInStaticallySizedGrammar(val.t[i], t[i])
+        
+      case SSGTaggedUnion(cases) =>
+        && val.SSVCase?
+        && (val.c as int) < |cases|
+        && StaticallySizedValInStaticallySizedGrammar(val.casev, cases[val.c])
+        
+      case SSGPadded(size, delt) =>
+        && val.SSVPadded?
+        && ValInGrammar(val.padv, delt)
+        && SizeOfV(val.padv, delt) <= size
+  }
 
-datatype V =
-           | StaticallySizedValue(v: StaticallySizedValue)
-           | VArray(a:seq<V>)
-           | VSSArray(sa:seq<StaticallySizedValue>)
-           | VTuple(t:seq<V>)
-           | VByteArray(b:seq<byte>)
-           | VUint32Array(va:seq<uint32>)
-           | VUint64Array(ua:seq<uint64>)
-           | VCase(c:uint64, val:V)
+  predicate ValInGrammar(val:DynamicallySizedValue, grammar:DynamicallySizedGrammar)
+    decreases grammar, val, 0
+  {
+    match grammar
+      case GArray(elt) => val.VArray? && forall v :: v in val.a ==> ValInGrammar(v, elt)
+      case GSSArray(selt) => val.VSSArray? && forall v :: v in val.sa ==> StaticallySizedValInStaticallySizedGrammar(v, selt)
+      case GTuple(t) =>
+        && val.VTuple?
+        && |t| == |val.t|
+        && forall i :: 0 <= i < |t| ==> ValInGrammar(val.t[i], t[i])
+      case GByteArray => val.VByteArray?
+      case GUint32Array => val.VUint32Array?
+      case GUint64Array => val.VUint64Array?
+      case GTaggedUnion(cases) =>
+        && val.VCase?
+        && (val.c as int) < |cases| &&
+        ValInGrammar(val.val, cases[val.c])
+  }
 
-function SizeOfStaticallySizedGrammarSeq(grammars: seq<StaticallySizedGrammar>) : nat
-{
-  if |grammars| == 0 then 0
-  else SizeOfStaticallySizedGrammarSeq(grammars[..|grammars|-1]) + SizeOfStaticallySizedGrammar(grammars[|grammars|-1])
-}
+  function parse_Uint32(data:seq<byte>, offset: nat) : (Option<StaticallySizedValue>, nat)
+    requires |data| < 0x1_0000_0000_0000_0000;
+  {
+    if offset + Uint32Size() as nat <= |data| then
+      (Some(SSVUint32(unpack_LittleEndian_Uint32(data[offset..offset+Uint32Size() as nat]))), offset + Uint32Size() as nat)
+    else
+      (None, offset)
+  }
 
-function MaxStaticallySizedGrammar(grammars: seq<StaticallySizedGrammar>) : nat
-{
-  if |grammars| == 0 then 0
-  else
-    var prefixMax := SizeOfStaticallySizedGrammarSeq(grammars[..|grammars|-1]);
-    var last := SizeOfStaticallySizedGrammar(grammars[|grammars|-1]);
-    if prefixMax < last then last
-    else prefixMax
-}
+  function parse_Uint64(data:seq<byte>, offset: nat) : (Option<StaticallySizedValue>, nat)
+    requires |data| < 0x1_0000_0000_0000_0000;
+  {
+    if offset + Uint64Size() as nat <= |data| then
+      (Some(SSVUint64(unpack_LittleEndian_Uint64(data[offset..offset+Uint64Size() as nat]))), offset + Uint64Size() as nat)
+    else
+      (None, offset)
+  }
 
-function SizeOfStaticallySizedGrammar(grammar: StaticallySizedGrammar) : nat
-{
-  match grammar
-    case SSGUint32 => 4
-    case SSGUint64 => 8
-    case SSGArray(len, elt) =>  len * SizeOfStaticallySizedGrammar(elt)
-    case SSGTuple(t, names) =>  SizeOfStaticallySizedGrammarSeq(t)
-    case SSGByteArray(len)   => len
-    case SSGUint32Array(len) => 4 * len
-    case SSGUint64Array(len) => 8 * len
-    case SSGTaggedUnion(cases, names) => MaxStaticallySizedGrammar(cases)
-    case SSGPadded(size, delt) => size
-}
+  method ParseUint32(data:seq<byte>, index:uint64) returns (value: Option<StaticallySizedValue>, rest_index:uint64)
+    requires |data| < 0x1_0000_0000_0000_0000;
+    requires (index as int) <= |data|
+    ensures (value, rest_index as nat) == parse_Uint32(data, index as nat)
+  {
+    if |data| as uint64 - index >= Uint32Size() {
+      var result := Unpack_LittleEndian_Uint32(data, index);
+      value := Some(SSVUint32(result));
+      rest_index := index + Uint32Size();
+    } else {
+      value := None;
+      rest_index := index;
+    }
+  }
 
-function SizeOfVSeq(vals: seq<V>, grammar: G) : nat
-  requires forall i | 0 <= i < |vals| :: ValInGrammar(vals[i], grammar)
-  decreases grammar, vals, 1
-{
-  if |vals| == 0 then 0
-  else SizeOfVSeq(vals[..|vals|-1], grammar) + SizeOfV(vals[|vals|-1], grammar)
-}
+  method ParseUint64(data:seq<byte>, index:uint64) returns (value: Option<StaticallySizedValue>, rest_index:uint64)
+    requires |data| < 0x1_0000_0000_0000_0000;
+    requires (index as int) <= |data|
+    ensures (value, rest_index as nat) == parse_Uint64(data, index as nat)
+  {
+    if |data| as uint64 - index >= Uint64Size() {
+      var result := Unpack_LittleEndian_Uint64(data, index);
+      value := Some(SSVUint64(result));
+      rest_index := index + Uint64Size();
+    } else {
+      value := None;
+      rest_index := index;
+    }
+  }
 
-function SizeOfVGSeq(vals: seq<V>, grammars: seq<G>) : nat
-  requires |vals| == |grammars|
-  requires forall i | 0 <= i < |vals| :: ValInGrammar(vals[i], grammars[i])
-  decreases grammars, vals, 1
-{
-  if |vals| == 0 then 0
-  else SizeOfVGSeq(vals[..|vals|-1], grammars[..|grammars|-1]) + SizeOfV(vals[|vals|-1], grammars[|grammars|-1])
-}
 
-function SizeOfV(val:V, grammar: G) : nat
-  requires ValInGrammar(val, grammar)
-  decreases grammar, val, 1
-{
-  match grammar
-    case StaticallySizedElement(g) => SizeOfStaticallySizedGrammar(g)
-    case GArray(elt)    => 8 + 8 * |val.a| + SizeOfVSeq(val.a, elt)
-    case GSSArray(selt) => |val.sa| * SizeOfStaticallySizedGrammar(selt)
-    case GTuple(t)      => 8 * |t| + SizeOfVGSeq(val.t, t)
-    case GByteArray     => |val.b|
-    case GUint32Array   => 4 * |val.va|
-    case GUint64Array   => 8 * |val.ua|
-    case GTaggedUnion(cases) => 8 + SizeOfV(val.val, cases[val.c])
-}
-           
-predicate StaticallySizedValInStaticallySizedGrammar(val:StaticallySizedValue, grammar:StaticallySizedGrammar)
-  decreases grammar, val, 1
-{
-  match grammar
-    case SSGUint32 => val.SSVUint32?
-    case SSGUint64 => val.SSVUint64?
-    case SSGArray(len, elt) =>
-      && val.SSVArray?
-      && |val.a| == len
-      && (forall v :: v in val.a ==> StaticallySizedValInStaticallySizedGrammar(v, grammar.elt))
-    case SSGTuple(t, names) =>
-      && val.SSVTuple?
-      && |val.t| == |t|
-      && forall i :: 0 <= i < |t| ==> StaticallySizedValInStaticallySizedGrammar(val.t[i], t[i])
-      
-    case SSGByteArray(len)   => val.SSVByteArray? && |val.b| == len
-    case SSGUint32Array(len) => val.SSVUint32Array? && |val.va| == len
-    case SSGUint64Array(len) => val.SSVUint64Array? && |val.ua| == len
-
-    case SSGTaggedUnion(cases, names) =>
-      && val.SSVCase?
-      && (val.c as int) < |cases|
-      && StaticallySizedValInStaticallySizedGrammar(val.casev, cases[val.c])
-    case SSGPadded(size, delt) =>
-      && val.SSVPadded?
-      && ValInGrammar(val.padv, delt)
-      && SizeOfV(val.padv, delt) <= size
-}
-
-predicate ValInGrammar(val:V, grammar:G)
-  decreases grammar, val, 0
-{
-  match grammar
-    case StaticallySizedElement(g) => val.StaticallySizedValue? && StaticallySizedValInStaticallySizedGrammar(val.v, g)
-    case GArray(elt) => val.VArray? && forall v :: v in val.a ==> ValInGrammar(v, elt)
-    case GSSArray(selt) => val.VSSArray? && forall v :: v in val.sa ==> StaticallySizedValInStaticallySizedGrammar(v, selt)
-    case GTuple(t) =>
-      && val.VTuple?
-      && |t| == |val.t|
-      && forall i :: 0 <= i < |t| ==> ValInGrammar(val.t[i], t[i])
-    case GByteArray => val.VByteArray?
-    case GUint32Array => val.VUint32Array?
-    case GUint64Array => val.VUint64Array?
-    case GTaggedUnion(cases) =>
-      && val.VCase?
-      && (val.c as int) < |cases| &&
-      ValInGrammar(val.val, cases[val.c])
-}
-
+  
 }
